ch 3 demo, refine exercise04

chapter03/exercises/exercise04.dfy
@@ -1,6 +1,30 @@
-Your goal is to model a lock service that consists of a single server and an arbitrary number of clients. The server provides the functionality of an exclusive lock. Initially, the server holds the lock. A client can acquire the lock (if the lock is currently held by the server) or it can return the lock (if it currently holds it). 
+// Your goal is to model a lock service that consists of a single server and an
+// arbitrary number of clients. The server provides the functionality of an
+// exclusive lock. Initially, the server holds the lock. A client can acquire
+// the lock (if the lock is currently held by the server) or it can return the
+// lock (if it currently holds it). 
+//
+// Do not model the network. Instead, model the beliefs of the server and each
+// of the clients, and allow steps that update a pair of (server, some client)
+// simultaneously (skipping the network asynchrony).
+//
+// Your state machine should reflect the state of the entire distributed system;
+// so it’s OK to have a single transition that atomically modifies the state of
+// multiple nodes in the system. 
 
-Do not model the network. 
+// Here's a helpful boilerplate for the inductive proof structure.
 
-Your state machine should reflect the state of the entire distributed system; so it’s OK to have a single transition that atomically modifies the state of multiple nodes in the system. 
+predicate Safety(s:Library) {
+  true  // Change me to the important property!
+}
 
+predicate Inv(s: Library) {
+  Safety(s)
+}
+
+lemma SafetyProof()
+  ensures forall s :: Init(s) ==> Inv(s)
+  ensures forall s, s' :: Inv(s) && Next(s, s') ==> Inv(s')
+  ensures forall s :: Inv(s) ==> Safety(s)
+{
+}
