chapter03/demos/demo00.dfy
@@ -1,0 +1,98 @@
+datatype Card = Shelf | Patron(name: string)
+datatype Book = Book(title: string)
+type Library = map<Book, Card>
+
+predicate Init(s: Library) {
+  forall book | book in s :: s[book] == Shelf
+}
+
+predicate CheckOut(s:Library, s':Library, book:Book, patron:string) {
+  && book in s
+  && s[book] == Shelf
+  && (forall book | book in s :: s[book] != Patron(patron))
+  && s' == s[book := Patron(patron)]
+}
+
+predicate CheckIn(s:Library, s':Library, book:Book, patron:string) {
+  && book in s
+  && s[book] == Patron(patron)
+  && s' == s[book := Shelf]
+}
+
+predicate Next(s:Library, s':Library) {
+  || (exists book, patron :: CheckOut(s, s', book, patron))
+  || (exists book, patron :: CheckIn(s, s', book, patron))
+}
+
+
+
+// name has at most book checked out.
+//
+// If you're coming from TLA+ background, you might have written
+// this using set cardinality:
+//   |BooksOutstanding(s, name)| <= 1
+// For a solution like that, see demo00_alternate.dfy.
+predicate CheckedOutTo(s:Library, book:Book, name: string) {
+  && book in s
+  && s[book] == Patron(name)
+}
+
+predicate HasAtMostOneBook(s: Library, name: string) {
+  forall book1, book2 ::
+    ( CheckedOutTo(s, book1, name) && CheckedOutTo(s, book2, name)
+      ==> book1 == book2 )
+}
+
+predicate Safety(s:Library) {
+  forall name :: HasAtMostOneBook(s, name)
+}
+
+predicate Inv(s: Library) {
+  Safety(s)
+}
+
+lemma SafetyProof()
+  ensures forall s :: Init(s) ==> Inv(s)
+  ensures forall s, s' :: Inv(s) && Next(s, s') ==> Inv(s')
+  ensures forall s :: Inv(s) ==> Safety(s)
+{
+  forall s, s' | Inv(s) && Next(s, s') ensures Inv(s') {
+    InductiveStep(s, s');
+  }
+}
+
+
+lemma InductiveStep(s: Library, s': Library)
+  requires Inv(s)
+  requires Next(s, s')
+  ensures Inv(s')
+{
+  forall name ensures HasAtMostOneBook(s', name)
+  {
+    assert HasAtMostOneBook(s, name);
+    if book, patron :| CheckOut(s, s', book, patron) {
+      forall book1, book2
+        | CheckedOutTo(s', book1, name) && CheckedOutTo(s', book2, name)
+        ensures book1 == book2
+      {
+        if !CheckedOutTo(s, book1, name) {
+          assert book1 == book;
+        }
+        if !CheckedOutTo(s, book2, name) {
+          assert book2 == book;
+        }
+      }
+      assert HasAtMostOneBook(s', name);
+    } else {
+      var book, patron :| CheckIn(s, s', book, patron);
+      forall book1, book2
+        | CheckedOutTo(s', book1, name) && CheckedOutTo(s', book2, name)
+        ensures book1 == book2
+      {
+        assert CheckedOutTo(s, book1, name);
+        assert CheckedOutTo(s, book2, name);
+      }
+      assert HasAtMostOneBook(s', name);
+    }
+  }
+}
