chapter03/demos/demo00_alternate.dfy
@@ -1,0 +1,150 @@
+datatype Card = Shelf | Patron(name: string)
+datatype Book = Book(title: string)
+type Library = map<Book, Card>
+
+predicate Init(s: Library) {
+  forall book | book in s :: s[book] == Shelf
+}
+
+predicate CheckOut(s:Library, s':Library, book:Book, patron:string) {
+  && book in s
+  && s[book] == Shelf
+  && (forall book | book in s :: s[book] != Patron(patron))
+  && s' == s[book := Patron(patron)]
+}
+
+predicate CheckIn(s:Library, s':Library, book:Book, patron:string) {
+  && book in s
+  && s[book] == Patron(patron)
+  && s' == s[book := Shelf]
+}
+
+predicate Next(s:Library, s':Library) {
+  || (exists book, patron :: CheckOut(s, s', book, patron))
+  || (exists book, patron :: CheckIn(s, s', book, patron))
+}
+
+predicate CheckedOutTo(s:Library, book:Book, name: string) {
+  && book in s
+  && s[book] == Patron(name)
+}
+
+function BooksOutstanding(s:Library, name: string) : set<Book> {
+  set book: Book | book in s && CheckedOutTo(s, book, name)
+}
+
+// This alternate variant uses set-cardinality as the definition
+// of the safety property.
+predicate Safety(s:Library) {
+  forall name :: |BooksOutstanding(s, name)| <= 1
+}
+
+predicate Inv(s: Library) {
+  Safety(s)
+}
+
+lemma SafetyProof()
+  ensures forall s :: Init(s) ==> Inv(s)
+  ensures forall s, s' :: Inv(s) && Next(s, s') ==> Inv(s')
+  ensures forall s :: Inv(s) ==> Safety(s)
+{
+  forall s, s' | Inv(s) && Next(s, s') ensures Inv(s') {
+    InductiveStep(s, s');
+  }
+}
+
+predicate HasAtMostOneBook(s: Library, name: string) {
+  forall book1, book2 ::
+    ( CheckedOutTo(s, book1, name) && CheckedOutTo(s, book2, name)
+      ==> book1 == book2 )
+}
+
+// ...But reasoning about set cardinality is a bit more annoying in
+// Dafny. Dafny's pretty darn good with quantifiers, but has a harder
+// time with set cardinality rules (details on why on Friday, at the
+// end of the course). So the way I chose to prove this version was
+// to show that the two definitions are equivalent...
+lemma SafetySynonyms(s: Library, name: string)
+  ensures (|BooksOutstanding(s, name)| <= 1) <==> HasAtMostOneBook(s, name)
+{
+  if |BooksOutstanding(s, name)| <= 1 {
+    if book1, book2 :|
+      CheckedOutTo(s, book1, name) && CheckedOutTo(s, book2, name)
+      && book1 != book2 {
+//      assert book1 in BooksOutstanding(s, name);
+//      assert book2 in BooksOutstanding(s, name);
+//      assert {book1, book2} <= BooksOutstanding(s, name);
+      subsetCardinality({book1, book2}, BooksOutstanding(s, name));
+//      assert |{book1, book2}| <= |BooksOutstanding(s, name)|;
+      assert false;
+    }
+  }
+  if HasAtMostOneBook(s, name) && |BooksOutstanding(s, name)| > 1 {
+    var uniqueBook :| CheckedOutTo(s, uniqueBook, name);
+    var remainingBooks := BooksOutstanding(s, name) - {uniqueBook};
+    assert |remainingBooks| > 0;  // tickle set cardinality relation.
+//    var otherBook :| otherBook in remainingBooks;
+//    assert false;
+  }
+}
+
+// ...and then invoke that lemma in the same basic proof structure as
+// in the first case. Perhaps you could write a proof that worked just
+// on the set definition?
+lemma InductiveStep(s: Library, s': Library)
+  requires Inv(s)
+  requires Next(s, s')
+  ensures Inv(s')
+{
+  forall name ensures |BooksOutstanding(s', name)| <= 1
+  {
+    SafetySynonyms(s, name);
+    assert HasAtMostOneBook(s, name);
+    if book, patron :| CheckOut(s, s', book, patron) {
+      forall book1, book2
+        | CheckedOutTo(s', book1, name) && CheckedOutTo(s', book2, name)
+        ensures book1 == book2
+      {
+        if !CheckedOutTo(s, book1, name) {
+          assert book1 == book;
+        }
+        if !CheckedOutTo(s, book2, name) {
+          assert book2 == book;
+        }
+      }
+      assert HasAtMostOneBook(s', name);
+    } else {
+      var book, patron :| CheckIn(s, s', book, patron);
+      forall book1, book2
+        | CheckedOutTo(s', book1, name) && CheckedOutTo(s', book2, name)
+        ensures book1 == book2
+      {
+        assert CheckedOutTo(s, book1, name);
+        assert CheckedOutTo(s, book2, name);
+      }
+      assert HasAtMostOneBook(s', name);
+    }
+    SafetySynonyms(s', name);
+  }
+}
+
+// Dafny seems to be missing a heuristic to trigger this cardinality relation!
+// So I proved it. This should get fixed in dafny, or at least tucked into a
+// library! How embarrassing.
+lemma subsetCardinality<T>(a:set<T>, b:set<T>)
+  requires a <= b
+  ensures |a| <= |b|
+{
+  if a == {} {
+    assert |a| <= |b|;
+  } else {
+    var e :| e in a;
+    if e in b {
+      subsetCardinality(a - {e}, b - {e});
+      assert |a| <= |b|;
+    } else {
+      subsetCardinality(a - {e}, b);
+      assert |a| <= |b|;
+    }
+  }
+}
